Refactoring the type system : every type gets its own file. Some trivial ones are defined somewhere else where it make the most sense.

theories/typing/perm.v
@@ -1,16 +1,12 @@
 From iris.proofmode Require Import tactics.
 From lrust.typing Require Export type.
-From lrust.lang Require Export proofmode.
-From lrust.lifetime Require Import frac_borrow.
-
-Delimit Scope perm_scope with P.
-Bind Scope perm_scope with perm.
-
-Module Perm.
+From lrust.lang Require Export proofmode notation.
+From lrust.lifetime Require Import borrow frac_borrow.
 
 Section perm.
-
   Context `{iris_typeG Σ}.
+
+  Definition perm {Σ} := thread_id → iProp Σ.
 
   Fixpoint eval_expr (ν : expr) : option val :=
     match ν with
@@ -47,11 +43,18 @@ Section perm.
   Global Instance top : Top (@perm Σ) :=
     λ _, True%I.
 
+  Definition perm_incl (ρ1 ρ2 : perm) :=
+    ∀ tid, lft_ctx -∗ ρ1 tid ={⊤}=∗ ρ2 tid.
+
+  Global Instance perm_equiv : Equiv perm :=
+    λ ρ1 ρ2, perm_incl ρ1 ρ2 ∧ perm_incl ρ2 ρ1.
+
+  Definition borrowing κ (ρ ρ1 ρ2 : perm) :=
+    ∀ tid, lft_ctx -∗ ρ tid -∗ ρ1 tid ={⊤}=∗ ρ2 tid ∗ extract κ ρ1 tid.
 End perm.
 
-End Perm.
-
-Import Perm.
+Delimit Scope perm_scope with P.
+Bind Scope perm_scope with perm.
 
 Notation "ν ◁ ty" := (has_type ν%E ty)
   (at level 75, right associativity) : perm_scope.
@@ -70,15 +73,21 @@ Notation "∃ x .. y , P" :=
 
 Infix "∗" := sep (at level 80, right associativity) : perm_scope.
 
-Section duplicable.
+Infix "⇒" := perm_incl (at level 95, no associativity) : C_scope.
+Notation "(⇒)" := perm_incl (only parsing) : C_scope.
 
+Notation "ρ1 ⇔ ρ2" := (equiv (A:=perm) ρ1%P ρ2%P)
+   (at level 95, no associativity) : C_scope.
+Notation "(⇔)" := (equiv (A:=perm)) (only parsing) : C_scope.
+
+Section duplicable.
   Context `{iris_typeG Σ}.
 
   Class Duplicable (ρ : @perm Σ) :=
     duplicable_persistent tid : PersistentP (ρ tid).
   Global Existing Instance duplicable_persistent.
 
-  Global Instance has_type_dup v ty : ty.(ty_dup) → Duplicable (v ◁ ty).
+  Global Instance has_type_dup v ty : Copy ty → Duplicable (v ◁ ty).
   Proof. intros Hdup tid. apply _. Qed.
 
   Global Instance lft_incl_dup κ κ' : Duplicable (κ ⊑ κ').
@@ -90,12 +99,9 @@ Section duplicable.
 
   Global Instance top_dup : Duplicable ⊤.
   Proof. intros tid. apply _. Qed.
-
 End duplicable.
 
-
 Section has_type.
-
   Context `{iris_typeG Σ}.
 
   Lemma has_type_value (v : val) ty tid :
@@ -121,5 +127,95 @@ Section has_type.
     - wp_bind e. simpl in EQν. destruct (eval_expr e) as [[[|l|]|]|]; try done.
       iApply ("IH" with "[] [HΦ]"). done. simpl. wp_op. inversion EQν. eauto.
   Qed.
-
 End has_type.
+
+Section perm_incl.
+  Context `{iris_typeG Σ}.
+
+  (* Properties *)
+  Global Instance perm_incl_preorder : PreOrder (⇒).
+  Proof.
+    split.
+    - iIntros (? tid) "H". eauto.
+    - iIntros (??? H12 H23 tid) "#LFT H". iApply (H23 with "LFT >").
+      by iApply (H12 with "LFT").
+  Qed.
+
+  Global Instance perm_equiv_equiv : Equivalence (⇔).
+  Proof.
+    split.
+    - by split.
+    - by intros x y []; split.
+    - intros x y z [] []. split; by transitivity y.
+  Qed.
+
+  Global Instance perm_incl_proper :
+    Proper ((⇔) ==> (⇔) ==> iff) (⇒).
+  Proof. intros ??[??]??[??]; split; intros ?; by simplify_order. Qed.
+
+  Global Instance perm_sep_proper :
+    Proper ((⇔) ==> (⇔) ==> (⇔)) (sep).
+  Proof.
+    intros ??[A B]??[C D]; split; iIntros (tid) "#LFT [A B]".
+    iMod (A with "LFT A") as "$". iApply (C with "LFT B").
+    iMod (B with "LFT A") as "$". iApply (D with "LFT B").
+  Qed.
+
+  Lemma uPred_equiv_perm_equiv ρ θ : (∀ tid, ρ tid ⊣⊢ θ tid) → (ρ ⇔ θ).
+  Proof. intros Heq. split=>tid; rewrite Heq; by iIntros. Qed.
+
+  Lemma perm_incl_top ρ : ρ ⇒ ⊤.
+  Proof. iIntros (tid) "H". eauto. Qed.
+
+  Lemma perm_incl_frame_l ρ ρ1 ρ2 : ρ1 ⇒ ρ2 → ρ ∗ ρ1 ⇒ ρ ∗ ρ2.
+  Proof. iIntros (Hρ tid) "#LFT [$?]". by iApply (Hρ with "LFT"). Qed.
+
+  Lemma perm_incl_frame_r ρ ρ1 ρ2 :
+    ρ1 ⇒ ρ2 → ρ1 ∗ ρ ⇒ ρ2 ∗ ρ.
+  Proof. iIntros (Hρ tid) "#LFT [?$]". by iApply (Hρ with "LFT"). Qed.
+
+  Lemma perm_incl_exists_intro {A} P x : P x ⇒ ∃ x : A, P x.
+  Proof. iIntros (tid) "_ H!>". by iExists x. Qed.
+
+  Global Instance perm_sep_assoc : Assoc (⇔) sep.
+  Proof. intros ???; split. by iIntros (tid) "_ [$[$$]]". by iIntros (tid) "_ [[$$]$]". Qed.
+
+  Global Instance perm_sep_comm : Comm (⇔) sep.
+  Proof. intros ??; split; by iIntros (tid) "_ [$$]". Qed.
+
+  Global Instance perm_top_right_id : RightId (⇔) ⊤ sep.
+  Proof. intros ρ; split. by iIntros (tid) "_ [? _]". by iIntros (tid) "_ $". Qed.
+
+  Global Instance perm_top_left_id : LeftId (⇔) ⊤ sep.
+  Proof. intros ρ. by rewrite comm right_id. Qed.
+
+  Lemma perm_incl_duplicable ρ (_ : Duplicable ρ) : ρ ⇒ ρ ∗ ρ.
+  Proof. iIntros (tid) "_ #H!>". by iSplit. Qed.
+
+  Lemma perm_tok_plus κ q1 q2 :
+    tok κ q1 ∗ tok κ q2 ⇔ tok κ (q1 + q2).
+  Proof. rewrite /tok /sep /=; split; by iIntros (tid) "_ [$$]". Qed.
+
+  Lemma perm_lftincl_refl κ : ⊤ ⇒ κ ⊑ κ.
+  Proof. iIntros (tid) "_ _!>". iApply lft_incl_refl. Qed.
+
+  Lemma perm_lftincl_trans κ1 κ2 κ3 : κ1 ⊑ κ2 ∗ κ2 ⊑ κ3 ⇒ κ1 ⊑ κ3.
+  Proof. iIntros (tid) "_ [#?#?]!>". iApply (lft_incl_trans with "[] []"); auto. Qed.
+
+  Lemma borrowing_perm_incl κ ρ ρ1 ρ2 θ :
+    borrowing κ ρ ρ1 ρ2 → ρ ∗ κ ∋ θ ∗ ρ1 ⇒ ρ2 ∗ κ ∋ (θ ∗ ρ1).
+  Proof.
+    iIntros (Hbor tid) "LFT (Hρ&Hθ&Hρ1)". iMod (Hbor with "LFT Hρ Hρ1") as "[$ Hρ1]".
+    iIntros "!>#H†". iSplitL "Hθ". by iApply "Hθ". by iApply "Hρ1".
+  Qed.
+
+  Lemma lftincl_borrowing κ κ' q : borrowing κ ⊤ q.[κ'] (κ ⊑ κ').
+  Proof.
+    iIntros (tid) "#LFT _ Htok". iApply (fupd_mask_mono (↑lftN)). done.
+    iMod (bor_create with "LFT [$Htok]") as "[Hbor Hclose]". done.
+    iMod (bor_fracture (λ q', (q * q').[κ'])%I with "LFT [Hbor]") as "Hbor". done.
+    { by rewrite Qp_mult_1_r. }
+    iSplitL "Hbor". iApply (frac_bor_incl with "LFT Hbor").
+    iIntros "!>H". by iMod ("Hclose" with "H") as ">$".
+  Qed.
+End perm_incl.
