theories/typing/type.v
@@ -1,8 +1,5 @@
-From Coq Require Import Qcanon.
-From iris.base_logic Require Import big_op.
 From iris.base_logic.lib Require Export na_invariants.
-From iris.program_logic Require Import hoare.
-From lrust.lang Require Export heap notation.
+From lrust.lang Require Import heap.
 From lrust.lifetime Require Import borrow frac_borrow reborrow.
 
 Class iris_typeG Σ := Iris_typeG {
@@ -15,469 +12,97 @@ Class iris_typeG Σ := Iris_typeG {
 Definition mgmtE := ↑lftN.
 Definition lrustN := nroot .@ "lrust".
 
-(* [perm] is defined here instead of perm.v in order to define [cont] *)
-Definition perm {Σ} := thread_id → iProp Σ.
-
 Section type.
+  Context `{iris_typeG Σ}.
 
-Context `{iris_typeG Σ}.
+  Record type :=
+    { ty_size : nat;
+      ty_own : thread_id → list val → iProp Σ;
+      ty_shr : lft → thread_id → coPset → loc → iProp Σ;
 
-Record type :=
-  { ty_size : nat;
-    ty_dup : bool;
-    ty_own : thread_id → list val → iProp Σ;
-    ty_shr : lft → thread_id → coPset → loc → iProp Σ;
+      ty_shr_persistent κ tid E l : PersistentP (ty_shr κ tid E l);
 
-    ty_dup_persistent tid vl : ty_dup → PersistentP (ty_own tid vl);
-    ty_shr_persistent κ tid E l : PersistentP (ty_shr κ tid E l);
+      ty_size_eq tid vl : ty_own tid vl -∗ ⌜length vl = ty_size⌝;
+      (* The mask for starting the sharing does /not/ include the
+         namespace N, for allowing more flexibility for the user of
+         this type (typically for the [own] type). AFAIK, there is no
+         fundamental reason for this.
 
-    ty_size_eq tid vl : ty_own tid vl -∗ ⌜length vl = ty_size⌝;
-    (* The mask for starting the sharing does /not/ include the
-       namespace N, for allowing more flexibility for the user of
-       this type (typically for the [own] type). AFAIK, there is no
-       fundamental reason for this.
+         This should not be harmful, since sharing typically creates
+         invariants, which does not need the mask.  Moreover, it is
+         more consistent with thread-local tokens, which we do not
+         give any. *)
+      ty_share E N κ l tid q : mgmtE ⊥ ↑N → mgmtE ⊆ E →
+        lft_ctx -∗ &{κ} (l ↦∗: ty_own tid) -∗ q.[κ] ={E}=∗ ty_shr κ tid (↑N) l ∗ q.[κ];
+      ty_shr_mono κ κ' tid E E' l : E ⊆ E' →
+        lft_ctx -∗ κ' ⊑ κ -∗ ty_shr κ tid E l -∗ ty_shr κ' tid E' l
+    }.
+  Global Existing Instances ty_shr_persistent.
 
-       This should not be harmful, since sharing typically creates
-       invariants, which does not need the mask.  Moreover, it is
-       more consistent with thread-local tokens, which we do not
-       give any. *)
-    ty_share E N κ l tid q : mgmtE ⊥ ↑N → mgmtE ⊆ E →
-      lft_ctx -∗ &{κ} (l ↦∗: ty_own tid) -∗ q.[κ] ={E}=∗ ty_shr κ tid (↑N) l ∗ q.[κ];
-    ty_shr_mono κ κ' tid E E' l : E ⊆ E' →
-      lft_ctx -∗ κ' ⊑ κ -∗ ty_shr κ tid E l -∗ ty_shr κ' tid E' l;
-    ty_shr_acc κ tid E F l q :
-      ty_dup → mgmtE ∪ F ⊆ E →
-      lft_ctx -∗ ty_shr κ tid F l -∗
-        q.[κ] ∗ na_own tid F ={E}=∗ ∃ q', ▷l ↦∗{q'}: ty_own tid ∗
-           (▷l ↦∗{q'}: ty_own tid ={E}=∗ q.[κ] ∗ na_own tid F)
+  Class Copy (t : type) := {
+    copy_persistent tid vl : PersistentP (t.(ty_own) tid vl);
+    copy_shr_acc κ tid E F l q :
+      mgmtE ∪ F ⊆ E →
+      lft_ctx -∗ t.(ty_shr) κ tid F l -∗
+        q.[κ] ∗ na_own tid F ={E}=∗ ∃ q', ▷l ↦∗{q'}: t.(ty_own) tid ∗
+          (▷l ↦∗{q'}: t.(ty_own) tid ={E}=∗ q.[κ] ∗ na_own tid F)
   }.
-Global Existing Instances ty_shr_persistent ty_dup_persistent.
+  Global Existing Instances copy_persistent.
 
-(* We are repeating the typeclass parameter here jsut to make sure
-   that simple_type does depend on it. Otherwise, the coercion defined
-   bellow will not be acceptable by Coq. *)
-Record simple_type `{iris_typeG Σ} :=
-  { st_size : nat;
-    st_own : thread_id → list val → iProp Σ;
+  (* We are repeating the typeclass parameter here jsut to make sure
+     that simple_type does depend on it. Otherwise, the coercion defined
+     bellow will not be acceptable by Coq. *)
+  Record simple_type `{iris_typeG Σ} :=
+    { st_size : nat;
+      st_own : thread_id → list val → iProp Σ;
 
-    st_size_eq tid vl : st_own tid vl -∗ ⌜length vl = st_size⌝;
-    st_own_persistent tid vl : PersistentP (st_own tid vl) }.
-Global Existing Instance st_own_persistent.
+      st_size_eq tid vl : st_own tid vl -∗ ⌜length vl = st_size⌝;
+      st_own_persistent tid vl : PersistentP (st_own tid vl) }.
 
-Program Definition ty_of_st (st : simple_type) : type :=
-  {| ty_size := st.(st_size); ty_dup := true;
-     ty_own := st.(st_own);
+  Global Existing Instance st_own_persistent.
 
-     (* [st.(st_own) tid vl] needs to be outside of the fractured
-        borrow, otherwise I do not know how to prove the shr part of
-        [lft_incl_ty_incl_shared_borrow]. *)
-     ty_shr := λ κ tid _ l,
-               (∃ vl, (&frac{κ} λ q, l ↦∗{q} vl) ∗ ▷ st.(st_own) tid vl)%I
-  |}.
-Next Obligation. intros. apply st_size_eq. Qed.
-Next Obligation.
-  intros st E N κ l tid q ? ?. iIntros "#LFT Hmt Htok".
-  iMod (bor_exists with "LFT Hmt") as (vl) "Hmt". set_solver.
-  iMod (bor_sep with "LFT Hmt") as "[Hmt Hown]". set_solver.
-  iMod (bor_persistent with "LFT Hown Htok") as "[Hown $]". set_solver.
-  iMod (bor_fracture with "LFT [Hmt]") as "Hfrac"; last first.
-  { iExists vl. by iFrame. }
-  done. set_solver.
-Qed.
-Next Obligation.
-  intros st κ κ' tid E E' l ?. iIntros "#LFT #Hord H".
-  iDestruct "H" as (vl) "[Hf Hown]".
-  iExists vl. iFrame. by iApply (frac_bor_shorten with "Hord").
-Qed.
-Next Obligation.
-  intros st κ tid E F l q ??. iIntros "#LFT #Hshr[Hlft $]".
-  iDestruct "Hshr" as (vl) "[Hf Hown]".
-  iMod (frac_bor_acc with "LFT Hf Hlft") as (q') "[Hmt Hclose]"; first set_solver.
-  iModIntro. iExists _. iDestruct "Hmt" as "[Hmt1 Hmt2]". iSplitL "Hmt1".
-  - iNext. iExists _. by iFrame.
-  - iIntros "Hmt1". iDestruct "Hmt1" as (vl') "[Hmt1 #Hown']".
-    iAssert (▷ ⌜length vl = length vl'⌝)%I as ">%".
-    { iNext.
-      iDestruct (st_size_eq with "Hown") as %->.
-      iDestruct (st_size_eq with "Hown'") as %->. done. }
-    iCombine "Hmt1" "Hmt2" as "Hmt". rewrite heap_mapsto_vec_op // Qp_div_2.
-    iDestruct "Hmt" as "[>% Hmt]". subst. by iApply "Hclose".
-Qed.
+  Program Definition ty_of_st (st : simple_type) : type :=
+    {| ty_size := st.(st_size); ty_own := st.(st_own);
 
+       (* [st.(st_own) tid vl] needs to be outside of the fractured
+          borrow, otherwise I do not know how to prove the shr part of
+          [lft_incl_ty_incl_shr_borrow]. *)
+       ty_shr := λ κ tid _ l,
+                 (∃ vl, (&frac{κ} λ q, l ↦∗{q} vl) ∗ ▷ st.(st_own) tid vl)%I
+    |}.
+  Next Obligation. intros. apply st_size_eq. Qed.
+  Next Obligation.
+    intros st E N κ l tid q ? ?. iIntros "#LFT Hmt Htok".
+    iMod (bor_exists with "LFT Hmt") as (vl) "Hmt". set_solver.
+    iMod (bor_sep with "LFT Hmt") as "[Hmt Hown]". set_solver.
+    iMod (bor_persistent with "LFT Hown Htok") as "[Hown $]". set_solver.
+    iMod (bor_fracture with "LFT [Hmt]") as "Hfrac"; last first.
+    { iExists vl. by iFrame. }
+    done. set_solver.
+  Qed.
+  Next Obligation.
+    intros st κ κ' tid E E' l ?. iIntros "#LFT #Hord H".
+    iDestruct "H" as (vl) "[Hf Hown]".
+    iExists vl. iFrame. by iApply (frac_bor_shorten with "Hord").
+  Qed.
+
+  Global Program Instance ty_of_st_copy st : Copy (ty_of_st st).
+  Next Obligation.
+    intros st κ tid E F l q ?. iIntros "#LFT #Hshr[Hlft $]".
+    iDestruct "Hshr" as (vl) "[Hf Hown]".
+    iMod (frac_bor_acc with "LFT Hf Hlft") as (q') "[Hmt Hclose]"; first set_solver.
+    iModIntro. iExists _. iDestruct "Hmt" as "[Hmt1 Hmt2]". iSplitL "Hmt1".
+    - iNext. iExists _. by iFrame.
+    - iIntros "Hmt1". iDestruct "Hmt1" as (vl') "[Hmt1 #Hown']".
+      iAssert (▷ ⌜length vl = length vl'⌝)%I as ">%".
+      { iNext. iDestruct (st_size_eq with "Hown") as %->.
+        iDestruct (st_size_eq with "Hown'") as %->. done. }
+      iCombine "Hmt1" "Hmt2" as "Hmt". rewrite heap_mapsto_vec_op // Qp_div_2.
+      iDestruct "Hmt" as "[>% Hmt]". subst. by iApply "Hclose".
+  Qed.
 End type.
 
 Coercion ty_of_st : simple_type >-> type.
 
-Hint Extern 0 (Is_true _.(ty_dup)) =>
-  exact I || assumption : typeclass_instances.
-
 Delimit Scope lrust_type_scope with T.
 Bind Scope lrust_type_scope with type.
-
-Module Types.
-Section types.
-
-  Context `{iris_typeG Σ}.
-
-  (* [emp] cannot be defined using [ty_of_st], because the least we
-     would be able to prove from its [ty_shr] would be [▷ False], but
-     we really need [False] to prove [ty_incl_emp]. *)
-  Program Definition emp :=
-    {| ty_size := 0; ty_dup := true;
-       ty_own tid vl := False%I; ty_shr κ tid E l := False%I |}.
-  Next Obligation. iIntros (tid vl) "[]". Qed.
-  Next Obligation.
-    iIntros (????????) "#LFT Hb Htok".
-    iMod (bor_exists with "LFT Hb") as (vl) "Hb". set_solver.
-    iMod (bor_sep with "LFT Hb") as "[_ Hb]". set_solver.
-    iMod (bor_persistent with "LFT Hb Htok") as "[>[] _]". set_solver.
-  Qed.
-  Next Obligation. intros. iIntros "_ _ []". Qed.
-  Next Obligation. intros. iIntros "_ []". Qed.
-
-  Program Definition unit : type :=
-    {| st_size := 0; st_own tid vl := ⌜vl = []⌝%I |}.
-  Next Obligation. iIntros (tid vl) "%". simpl. by subst. Qed.
-
-  Program Definition bool : type :=
-    {| st_size := 1; st_own tid vl := (∃ z:bool, ⌜vl = [ #z ]⌝)%I |}.
-  Next Obligation. iIntros (tid vl) "H". iDestruct "H" as (z) "%". by subst. Qed.
-
-  Program Definition int : type :=
-    {| st_size := 1; st_own tid vl := (∃ z:Z, ⌜vl = [ #z ]⌝)%I |}.
-  Next Obligation. iIntros (tid vl) "H". iDestruct "H" as (z) "%". by subst. Qed.
-
-  Program Definition own (q : Qp) (ty : type) :=
-    {| ty_size := 1; ty_dup := false;
-       ty_own tid vl :=
-         (* We put a later in front of the †{q}, because we cannot use
-            [ty_size_eq] on [ty] at step index 0, which would in turn
-            prevent us to prove [ty_incl_own].
-
-            Since this assertion is timeless, this should not cause
-            problems. *)
-         (∃ l:loc, ⌜vl = [ #l ]⌝ ∗ ▷ l ↦∗: ty.(ty_own) tid ∗ ▷ †{q}l…ty.(ty_size))%I;
-       ty_shr κ tid E l :=
-         (∃ l':loc, &frac{κ}(λ q', l ↦{q'} #l') ∗
-            □ (∀ q' F, ⌜E ∪ mgmtE ⊆ F⌝ →
-                 q'.[κ] ={F,F∖E}▷=∗ ty.(ty_shr) κ tid E l' ∗ q'.[κ]))%I
-    |}.
-  Next Obligation. done. Qed.
-  Next Obligation.
-    iIntros (q ty tid vl) "H". iDestruct "H" as (l) "[% _]". by subst.
-  Qed.
-  Next Obligation.
-    move=> q ty E N κ l tid q' ?? /=. iIntros "#LFT Hshr Htok".
-    iMod (bor_exists with "LFT Hshr") as (vl) "Hb". set_solver.
-    iMod (bor_sep with "LFT Hb") as "[Hb1 Hb2]". set_solver.
-    iMod (bor_exists with "LFT Hb2") as (l') "Hb2". set_solver.
-    iMod (bor_sep with "LFT Hb2") as "[EQ Hb2]". set_solver.
-    iMod (bor_persistent with "LFT EQ Htok") as "[>% $]". set_solver. subst.
-    rewrite heap_mapsto_vec_singleton.
-    iMod (bor_sep with "LFT Hb2") as "[Hb2 _]". set_solver.
-    iMod (bor_fracture (λ q, l ↦{q} #l')%I with "LFT Hb1") as "Hbf". set_solver.
-    rewrite bor_unfold_idx. iDestruct "Hb2" as (i) "(#Hpb&Hpbown)".
-    iMod (inv_alloc N _ (idx_bor_own 1 i ∨ ty_shr ty κ tid (↑N) l')%I
-         with "[Hpbown]") as "#Hinv"; first by eauto.
-    iExists l'. iIntros "!>{$Hbf}!#". iIntros (q'' F) "% Htok".
-    iMod (inv_open with "Hinv") as "[INV Hclose]". set_solver.
-    iDestruct "INV" as "[>Hbtok|#Hshr]".
-    - iMod (bor_later_tok with "LFT [Hbtok] Htok") as "H". set_solver.
-      { rewrite bor_unfold_idx. eauto. }
-      iModIntro. iNext. iMod "H" as "[Hb Htok]".
-      iMod (ty.(ty_share) with "LFT Hb Htok") as "[#$ $]". done. set_solver.
-      iApply "Hclose". auto.
-    - iModIntro. iNext. iMod ("Hclose" with "[]") as "_"; by eauto.
-  Qed.
-  Next Obligation.
-    intros _ ty κ κ' tid E E' l ?. iIntros "#LFT #Hκ #H".
-    iDestruct "H" as (l') "[Hfb #Hvs]".
-    iExists l'. iSplit. by iApply (frac_bor_shorten with "[]"). iIntros "!#".
-    iIntros (q' F) "% Htok".
-    iApply (step_fupd_mask_mono F _ _ (F∖E)). set_solver. set_solver.
-    iMod (lft_incl_acc with "Hκ Htok") as (q'') "[Htok Hclose]". set_solver.
-    iMod ("Hvs" with "* [%] Htok") as "Hvs'". set_solver. iModIntro. iNext.
-    iMod "Hvs'" as "[Hshr Htok]". iMod ("Hclose" with "Htok") as "$".
-      by iApply (ty.(ty_shr_mono) with "LFT Hκ").
-  Qed.
-  Next Obligation. done. Qed.
-
-  Program Definition uniq_bor (κ:lft) (ty:type) :=
-    {| ty_size := 1; ty_dup := false;
-       ty_own tid vl :=
-         (∃ l:loc, ⌜vl = [ #l ]⌝ ∗ &{κ} l ↦∗: ty.(ty_own) tid)%I;
-       ty_shr κ' tid E l :=
-         (∃ l':loc, &frac{κ'}(λ q', l ↦{q'} #l') ∗
-            □ ∀ q' F, ⌜E ∪ mgmtE ⊆ F⌝ → q'.[κ∪κ']
-               ={F, F∖E∖↑lftN}▷=∗ ty.(ty_shr) (κ∪κ') tid E l' ∗ q'.[κ∪κ'])%I
-    |}.
-  Next Obligation. done. Qed.
-  Next Obligation.
-    iIntros (q ty tid vl) "H". iDestruct "H" as (l) "[% _]". by subst.
-  Qed.
-  Next Obligation.
-    move=> κ ty E N κ' l tid q' ??/=. iIntros "#LFT Hshr Htok".
-    iMod (bor_exists with "LFT Hshr") as (vl) "Hb". set_solver.
-    iMod (bor_sep with "LFT Hb") as "[Hb1 Hb2]". set_solver.
-    iMod (bor_exists with "LFT Hb2") as (l') "Hb2". set_solver.
-    iMod (bor_sep with "LFT Hb2") as "[EQ Hb2]". set_solver.
-    iMod (bor_persistent with "LFT EQ Htok") as "[>% $]". set_solver. subst.
-    rewrite heap_mapsto_vec_singleton.
-    iMod (bor_fracture (λ q, l ↦{q} #l')%I with "LFT Hb1") as "Hbf". set_solver.
-    rewrite {1}bor_unfold_idx. iDestruct "Hb2" as (i) "[#Hpb Hpbown]".
-    iMod (inv_alloc N _ (idx_bor_own 1 i ∨ ty_shr ty (κ∪κ') tid (↑N) l')%I
-         with "[Hpbown]") as "#Hinv"; first by eauto.
-    iExists l'. iIntros "!>{$Hbf}!#". iIntros (q'' F) "% Htok".
-    iMod (inv_open with "Hinv") as "[INV Hclose]". set_solver.
-    iDestruct "INV" as "[>Hbtok|#Hshr]".
-    - iMod (bor_unnest _ _ _ (l' ↦∗: ty_own ty tid)%I with "LFT [Hbtok]") as "Hb".
-      { set_solver. } { iApply bor_unfold_idx. eauto. }
-      iModIntro. iNext. iMod "Hb".
-      iMod (ty.(ty_share) with "LFT Hb Htok") as "[#$ $]"; try done. set_solver.
-      iApply "Hclose". eauto.
-    - iMod ("Hclose" with "[]") as "_". by eauto.
-      iApply step_fupd_mask_mono; last by eauto. done. set_solver.
-  Qed.
-  Next Obligation.
-    intros κ0 ty κ κ' tid E E' l ?. iIntros "#LFT #Hκ #H".
-    iDestruct "H" as (l') "[Hfb Hvs]". iAssert (κ0∪κ' ⊑ κ0∪κ)%I as "#Hκ0".
-    { iApply (lft_incl_glb with "[] []").
-      - iApply lft_le_incl. apply gmultiset_union_subseteq_l.
-      - iApply (lft_incl_trans with "[] Hκ").
-        iApply lft_le_incl. apply gmultiset_union_subseteq_r. }
-    iExists l'. iSplit. by iApply (frac_bor_shorten with "[]").
-    iIntros "!#". iIntros (q F) "% Htok".
-    iApply (step_fupd_mask_mono F _ _ (F∖E∖ ↑lftN)). set_solver. set_solver.
-    iMod (lft_incl_acc with "Hκ0 Htok") as (q') "[Htok Hclose]". set_solver.
-    iMod ("Hvs" with "* [%] Htok") as "Hvs'". set_solver. iModIntro. iNext.
-    iMod "Hvs'" as "[#Hshr Htok]". iMod ("Hclose" with "Htok") as "$".
-      by iApply (ty_shr_mono with "LFT Hκ0").
-  Qed.
-  Next Obligation. done. Qed.
-
-  Program Definition shared_bor (κ : lft) (ty : type) : type :=
-    {| st_size := 1;
-       st_own tid vl :=
-         (∃ (l:loc), ⌜vl = [ #l ]⌝ ∗ ty.(ty_shr) κ tid (↑lrustN) l)%I |}.
-  Next Obligation.
-    iIntros (κ ty tid vl) "H". iDestruct "H" as (l) "[% _]". by subst.
-  Qed.
-
-  Lemma split_prod_mt tid ty1 ty2 q l :
-    (l ↦∗{q}: λ vl,
-       ∃ vl1 vl2, ⌜vl = vl1 ++ vl2⌝ ∗ ty1.(ty_own) tid vl1 ∗ ty2.(ty_own) tid vl2)%I
-       ⊣⊢ l ↦∗{q}: ty1.(ty_own) tid ∗ shift_loc l ty1.(ty_size) ↦∗{q}: ty2.(ty_own) tid.
-  Proof.
-    iSplit; iIntros "H".
-    - iDestruct "H" as (vl) "[H↦ H]". iDestruct "H" as (vl1 vl2) "(% & H1 & H2)".
-      subst. rewrite heap_mapsto_vec_app. iDestruct "H↦" as "[H↦1 H↦2]".
-      iDestruct (ty_size_eq with "H1") as %->.
-      iSplitL "H1 H↦1"; iExists _; iFrame.
-    - iDestruct "H" as "[H1 H2]". iDestruct "H1" as (vl1) "[H↦1 H1]".
-      iDestruct "H2" as (vl2) "[H↦2 H2]". iExists (vl1 ++ vl2).
-      rewrite heap_mapsto_vec_app. iDestruct (ty_size_eq with "H1") as %->.
-      iFrame. iExists _, _. by iFrame.
-  Qed.
-
-  Program Definition product2 (ty1 ty2 : type) :=
-    {| ty_size := ty1.(ty_size) + ty2.(ty_size);
-       ty_dup := ty1.(ty_dup) && ty2.(ty_dup);
-       ty_own tid vl := (∃ vl1 vl2,
-         ⌜vl = vl1 ++ vl2⌝ ∗ ty1.(ty_own) tid vl1 ∗ ty2.(ty_own) tid vl2)%I;
-       ty_shr κ tid E l :=
-         (∃ E1 E2, ⌜E1 ⊥ E2 ∧ E1 ⊆ E ∧ E2 ⊆ E⌝ ∗
-            ty1.(ty_shr) κ tid E1 l ∗
-            ty2.(ty_shr) κ tid E2 (shift_loc l ty1.(ty_size)))%I |}.
-  Next Obligation. intros ty1 ty2 tid vl [Hdup1 Hdup2]%andb_True. apply _. Qed.
-  Next Obligation.
-    iIntros (ty1 ty2 tid vl) "H". iDestruct "H" as (vl1 vl2) "(% & H1 & H2)".
-    subst. rewrite app_length !ty_size_eq.
-    iDestruct "H1" as %->. iDestruct "H2" as %->. done.
-  Qed.
-  Next Obligation.
-    intros ty1 ty2 E N κ l tid q ??. iIntros "#LFT /=H Htok".
-    rewrite split_prod_mt.
-    iMod (bor_sep with "LFT H") as "[H1 H2]". set_solver.
-    iMod (ty1.(ty_share) _ (N .@ 1) with "LFT H1 Htok") as "[? Htok]". solve_ndisj. done.
-    iMod (ty2.(ty_share) _ (N .@ 2) with "LFT H2 Htok") as "[? $]". solve_ndisj. done.
-    iModIntro. iExists (↑N .@ 1). iExists (↑N .@ 2). iFrame.
-    iPureIntro. split. solve_ndisj. split; apply nclose_subseteq.
-  Qed.
-  Next Obligation.
-    intros ty1 ty2 κ κ' tid E E' l ?. iIntros "#LFT /= #H⊑ H".
-    iDestruct "H" as (N1 N2) "(% & H1 & H2)". iExists N1, N2.
-    iSplit. iPureIntro. set_solver.
-    iSplitL "H1"; by iApply (ty_shr_mono with "LFT H⊑").
-  Qed.
-  Next Obligation.
-    intros ty1 ty2 κ tid E F l q [Hdup1 Hdup2]%andb_True ?.
-    iIntros "#LFT H[[Htok1 Htok2] Htl]". iDestruct "H" as (E1 E2) "(% & H1 & H2)".
-    assert (F = E1 ∪ E2 ∪ F∖(E1 ∪ E2)) as ->.
-    { rewrite -union_difference_L; set_solver. }
-    repeat setoid_rewrite na_own_union; first last.
-    set_solver. set_solver. set_solver. set_solver.
-    iDestruct "Htl" as "[[Htl1 Htl2] $]".
-    iMod (ty1.(ty_shr_acc) with "LFT H1 [$Htok1 $Htl1]") as (q1) "[H1 Hclose1]".
-      done. set_solver.
-    iMod (ty2.(ty_shr_acc) with "LFT H2 [$Htok2 $Htl2]") as (q2) "[H2 Hclose2]".
-      done. set_solver.
-    destruct (Qp_lower_bound q1 q2) as (qq & q'1 & q'2 & -> & ->). iExists qq.
-    iDestruct "H1" as (vl1) "[H↦1 H1]". iDestruct "H2" as (vl2) "[H↦2 H2]".
-    rewrite !split_prod_mt.
-    iAssert (▷ ⌜length vl1 = ty1.(ty_size)⌝)%I with "[#]" as ">%".
-    { iNext. by iApply ty_size_eq. }
-    iAssert (▷ ⌜length vl2 = ty2.(ty_size)⌝)%I with "[#]" as ">%".
-    { iNext. by iApply ty_size_eq. }
-    iDestruct "H↦1" as "[H↦1 H↦1f]". iDestruct "H↦2" as "[H↦2 H↦2f]".
-    iIntros "!>". iSplitL "H↦1 H1 H↦2 H2".
-    - iNext. iSplitL "H↦1 H1". iExists vl1. by iFrame. iExists vl2. by iFrame.
-    - iIntros "[H1 H2]".
-      iDestruct "H1" as (vl1') "[H↦1 H1]". iDestruct "H2" as (vl2') "[H↦2 H2]".
-      iAssert (▷ ⌜length vl1' = ty1.(ty_size)⌝)%I with "[#]" as ">%".
-      { iNext. by iApply ty_size_eq. }
-      iAssert (▷ ⌜length vl2' = ty2.(ty_size)⌝)%I with "[#]" as ">%".
-      { iNext. by iApply ty_size_eq. }
-      iCombine "H↦1" "H↦1f" as "H↦1". iCombine "H↦2" "H↦2f" as "H↦2".
-      rewrite !heap_mapsto_vec_op; try by congruence.
-      iDestruct "H↦1" as "[_ H↦1]". iDestruct "H↦2" as "[_ H↦2]".
-      iMod ("Hclose1" with "[H1 H↦1]") as "[$$]". by iExists _; iFrame.
-      iMod ("Hclose2" with "[H2 H↦2]") as "[$$]". by iExists _; iFrame. done.
-  Qed.
-
-  Definition product := fold_right product2 unit.
-
-  Lemma split_sum_mt l tid q tyl :
-    (l ↦∗{q}: λ vl,
-         ∃ (i : nat) vl', ⌜vl = #i :: vl'⌝ ∗ ty_own (nth i tyl emp) tid vl')%I
-    ⊣⊢ ∃ (i : nat), l ↦{q} #i ∗ shift_loc l 1 ↦∗{q}: ty_own (nth i tyl emp) tid.
-  Proof.
-    iSplit; iIntros "H".
-    - iDestruct "H" as (vl) "[Hmt Hown]". iDestruct "Hown" as (i vl') "[% Hown]".
-      subst. iExists i. iDestruct (heap_mapsto_vec_cons with "Hmt") as "[$ Hmt]".
-      iExists vl'. by iFrame.
-    - iDestruct "H" as (i) "[Hmt1 Hown]". iDestruct "Hown" as (vl) "[Hmt2 Hown]".
-      iExists (#i::vl). rewrite heap_mapsto_vec_cons. iFrame. eauto.
-  Qed.
-
-  Class LstTySize (n : nat) (tyl : list type) :=
-    size_eq : Forall ((= n) ∘ ty_size) tyl.
-  Instance LstTySize_nil n : LstTySize n nil := List.Forall_nil _.
-  Lemma LstTySize_cons n ty tyl :
-    ty.(ty_size) = n → LstTySize n tyl → LstTySize n (ty :: tyl).
-  Proof. intros. constructor; done. Qed.
-
-  Lemma sum_size_eq n tid i tyl vl {Hn : LstTySize n tyl} :
-    ty_own (nth i tyl emp) tid vl -∗ ⌜length vl = n⌝.
-  Proof.
-    iIntros "Hown". iDestruct (ty_size_eq with "Hown") as %->.
-    revert Hn. rewrite /LstTySize List.Forall_forall /= =>Hn.
-    edestruct nth_in_or_default as [| ->]. by eauto.
-    iDestruct "Hown" as "[]".
-  Qed.
-
-  Program Definition sum {n} (tyl : list type) {_:LstTySize n tyl} :=
-    {| ty_size := S n; ty_dup := forallb ty_dup tyl;
-       ty_own tid vl :=
-         (∃ (i : nat) vl', ⌜vl = #i :: vl'⌝ ∗ (nth i tyl emp).(ty_own) tid vl')%I;
-       ty_shr κ tid N l :=
-         (∃ (i : nat), (&frac{κ} λ q, l ↦{q} #i) ∗
-               (nth i tyl emp).(ty_shr) κ tid N (shift_loc l 1))%I
-    |}.
-  Next Obligation.
-    intros n tyl Hn tid vl Hdup%Is_true_eq_true.
-    cut (∀ i vl', PersistentP (ty_own (nth i tyl emp) tid vl')). apply _.
-    intros. apply ty_dup_persistent. edestruct nth_in_or_default as [| ->]; last done.
-    rewrite ->forallb_forall in Hdup. auto using Is_true_eq_left.
-  Qed.
-  Next Obligation.
-    iIntros (n tyl Hn tid vl) "Hown". iDestruct "Hown" as (i vl') "(%&Hown)".
-    subst. simpl. by iDestruct (sum_size_eq with "Hown") as %->.
-  Qed.
-  Next Obligation.
-    intros n tyl Hn E N κ l tid q ??. iIntros "#LFT Hown Htok". rewrite split_sum_mt.
-    iMod (bor_exists with "LFT Hown") as (i) "Hown". set_solver.
-    iMod (bor_sep with "LFT Hown") as "[Hmt Hown]". set_solver.
-    iMod ((nth i tyl emp).(ty_share) with "LFT Hown Htok") as "[#Hshr $]"; try done.
-    iMod (bor_fracture with "LFT [-]") as "H"; last by eauto. set_solver. iFrame.
-  Qed.
-  Next Obligation.
-    intros n tyl Hn κ κ' tid E E' l ?. iIntros "#LFT #Hord H".
-    iDestruct "H" as (i) "[Hown0 Hown]". iExists i. iSplitL "Hown0".
-    by iApply (frac_bor_shorten with "Hord").
-    iApply ((nth i tyl emp).(ty_shr_mono) with "LFT Hord"); last done. done.
-  Qed.
-  Next Obligation.
-    intros n tyl Hn κ tid E F l q Hdup%Is_true_eq_true ?.
-    iIntros "#LFT #H[[Htok1 Htok2] Htl]".
-    setoid_rewrite split_sum_mt. iDestruct "H" as (i) "[Hshr0 Hshr]".
-    iMod (frac_bor_acc with "LFT Hshr0 Htok1") as (q'1) "[Hown Hclose]". set_solver.
-    iMod ((nth i tyl emp).(ty_shr_acc) with "LFT Hshr [Htok2 $Htl]")
-      as (q'2) "[Hownq Hclose']"; try done.
-    { edestruct nth_in_or_default as [| ->]; last done.
-      rewrite ->forallb_forall in Hdup. auto using Is_true_eq_left. }
-    destruct (Qp_lower_bound q'1 q'2) as (q' & q'01 & q'02 & -> & ->).
-    rewrite -{1}heap_mapsto_vec_prop_op; last (by intros; apply sum_size_eq, Hn).
-    iDestruct "Hownq" as "[Hownq1 Hownq2]". iDestruct "Hown" as "[Hown1 Hown2]".
-    iExists q'. iModIntro. iSplitL "Hown1 Hownq1".
-    - iNext. iExists i. by iFrame.
-    - iIntros "H". iDestruct "H" as (i') "[Hown1 Hownq1]".
-      iCombine "Hown1" "Hown2" as "Hown". rewrite heap_mapsto_op.
-      iDestruct "Hown" as "[>#Hi Hown]". iDestruct "Hi" as %[= ->%Z_of_nat_inj].
-      iMod ("Hclose" with "Hown") as "$".
-      iCombine "Hownq1" "Hownq2" as "Hownq".
-      rewrite heap_mapsto_vec_prop_op; last (by intros; apply sum_size_eq, Hn).
-      by iApply "Hclose'".
-  Qed.
-
-  Program Definition uninit : type :=
-    {| st_size := 1; st_own tid vl := ⌜length vl = 1%nat⌝%I |}.
-  Next Obligation. done. Qed.
-
-  Program Definition cont {n : nat} (ρ : vec val n → @perm Σ) :=
-    {| ty_size := 1; ty_dup := false;
-       ty_own tid vl := (∃ f, ⌜vl = [f]⌝ ∗
-          ∀ vl, ρ vl tid -∗ na_own tid ⊤
-                 -∗ WP f (map of_val vl) {{λ _, False}})%I;
-       ty_shr κ tid N l := True%I |}.
-  Next Obligation. done. Qed.
-  Next Obligation.
-    iIntros (n ρ tid vl) "H". iDestruct "H" as (f) "[% _]". by subst.
-  Qed.
-  Next Obligation. intros. by iIntros "_ _ $". Qed.
-  Next Obligation. intros. by iIntros "_ _ _". Qed.
-  Next Obligation. done. Qed.
-
-  (* TODO : For now, functions are not Send. This means they cannot be
-     called in another thread than the one that created it.  We will
-     need Send functions when dealing with multithreading ([fork]
-     needs a Send closure). *)
-  Program Definition fn {A n} (ρ : A -> vec val n → @perm Σ) : type :=
-    {| st_size := 1;
-       st_own tid vl := (∃ f, ⌜vl = [f]⌝ ∗ ∀ x vl,
-         {{ ρ x vl tid ∗ na_own tid ⊤ }} f (map of_val vl) {{λ _, False}})%I |}.
-  Next Obligation.
-    iIntros (x n ρ tid vl) "H". iDestruct "H" as (f) "[% _]". by subst.
-  Qed.
-
-End types.
-
-End Types.
-
-Existing Instance Types.LstTySize_nil.
-Hint Extern 1 (Types.LstTySize _ (_ :: _)) =>
-  apply Types.LstTySize_cons; [compute; reflexivity|] : typeclass_instances.
-
-Import Types.
-
-Notation "∅" := emp : lrust_type_scope.
-Notation "&uniq{ κ } ty" := (uniq_bor κ ty)
-  (format "&uniq{ κ } ty", at level 20, right associativity) : lrust_type_scope.
-Notation "&shr{ κ } ty" := (shared_bor κ ty)
-  (format "&shr{ κ } ty", at level 20, right associativity) : lrust_type_scope.
-
-Arguments product : simpl never.
-Notation Π := product.
-(* Σ is commonly used for the current functor. So it cannot be defined
-   as Π for products. We stick to the following form. *)
-Notation "Σ[ ty1 ; .. ; tyn ]" :=
-  (sum (cons ty1 (..(cons tyn nil)..))) : lrust_type_scope.
