theories/typing/function.v
@@ -1,0 +1,121 @@
+From iris.proofmode Require Import tactics.
+From iris.program_logic Require Import hoare.
+From lrust.lifetime Require Import borrow.
+From lrust.typing Require Export type.
+From lrust.typing Require Import type_incl typing.
+
+Section fn.
+  Context `{iris_typeG Σ}.
+
+  Program Definition cont {n : nat} (ρ : vec val n → @perm Σ) :=
+    {| ty_size := 1;
+       ty_own tid vl := (∃ f, ⌜vl = [f]⌝ ∗
+          ∀ vl, ρ vl tid -∗ na_own tid ⊤
+                 -∗ WP f (map of_val vl) {{λ _, False}})%I;
+       ty_shr κ tid N l := True%I |}.
+  Next Obligation.
+    iIntros (n ρ tid vl) "H". iDestruct "H" as (f) "[% _]". by subst.
+  Qed.
+  Next Obligation. intros. by iIntros "_ _ $". Qed.
+  Next Obligation. intros. by iIntros "_ _ _". Qed.
+
+  (* TODO : For now, functions are not Send. This means they cannot be
+     called in another thread than the one that created it.  We will
+     need Send functions when dealing with multithreading ([fork]
+     needs a Send closure). *)
+  Program Definition fn {A n} (ρ : A -> vec val n → @perm Σ) : type :=
+    {| st_size := 1;
+       st_own tid vl := (∃ f, ⌜vl = [f]⌝ ∗ ∀ x vl,
+         {{ ρ x vl tid ∗ na_own tid ⊤ }} f (map of_val vl) {{λ _, False}})%I |}.
+  Next Obligation.
+    iIntros (x n ρ tid vl) "H". iDestruct "H" as (f) "[% _]". by subst.
+  Qed.
+
+  Lemma ty_incl_cont {n} ρ ρ1 ρ2 :
+    Duplicable ρ → (∀ vl : vec val n, ρ ∗ ρ2 vl ⇒ ρ1 vl) →
+    ty_incl ρ (cont ρ1) (cont ρ2).
+  Proof.
+    iIntros (? Hρ1ρ2 tid) "#LFT #Hρ!>". iSplit; iIntros "!#*H"; last by auto.
+    iDestruct "H" as (f) "[% Hwp]". subst. iExists _. iSplit. done.
+    iIntros (vl) "Hρ2 Htl". iApply ("Hwp" with ">[-Htl] Htl").
+    iApply (Hρ1ρ2 with "LFT"). by iFrame.
+  Qed.
+
+  Lemma ty_incl_fn {A n} ρ ρ1 ρ2 :
+    Duplicable ρ → (∀ (x : A) (vl : vec val n), ρ ∗ ρ2 x vl ⇒ ρ1 x vl) →
+    ty_incl ρ (fn ρ1) (fn ρ2).
+  Proof.
+    iIntros (? Hρ1ρ2 tid) "#LFT #Hρ!>". iSplit; iIntros "!#*#H".
+    - iDestruct "H" as (f) "[% Hwp]". subst. iExists _. iSplit. done.
+      iIntros (x vl) "!#[Hρ2 Htl]". iApply ("Hwp" with ">").
+      iFrame. iApply (Hρ1ρ2 with "LFT"). by iFrame.
+    - iSplit; last done. simpl. iDestruct "H" as (vl0) "[? Hvl]".
+      iExists vl0. iFrame "#". iNext. iDestruct "Hvl" as (f) "[% Hwp]".
+      iExists f. iSplit. done. iIntros (x vl) "!#[Hρ2 Htl]".
+      iApply ("Hwp" with ">"). iFrame. iApply (Hρ1ρ2 with "LFT >"). by iFrame.
+  Qed.
+
+  Lemma ty_incl_fn_cont {A n} ρ ρf (x : A) :
+    ty_incl ρ (fn ρf) (cont (n:=n) (ρf x)).
+  Proof.
+    iIntros (tid) "#LFT _!>". iSplit; iIntros "!#*H"; last by iSplit.
+    iDestruct "H" as (f) "[%#H]". subst. iExists _. iSplit. done.
+    iIntros (vl) "Hρf Htl". iApply "H". by iFrame.
+  Qed.
+
+  Lemma ty_incl_fn_specialize {A B n} (f : A → B) ρ ρfn :
+    ty_incl ρ (fn (n:=n) ρfn) (fn (ρfn ∘ f)).
+  Proof.
+    iIntros (tid) "_ _!>". iSplit; iIntros "!#*H".
+    - iDestruct "H" as (fv) "[%#H]". subst. iExists _. iSplit. done.
+      iIntros (x vl). by iApply "H".
+    - iSplit; last done.
+      iDestruct "H" as (fvl) "[?Hown]". iExists _. iFrame. iNext.
+      iDestruct "Hown" as (fv) "[%H]". subst. iExists _. iSplit. done.
+      iIntros (x vl). by iApply "H".
+  Qed.
+
+  Lemma typed_fn {A n} `{Duplicable _ ρ, Closed (f :b: xl +b+ []) e} θ :
+    length xl = n →
+    (∀ (a : A) (vl : vec val n) (fv : val) e',
+        subst_l xl (map of_val vl) e = Some e' →
+        typed_program (fv ◁ fn θ ∗ (θ a vl) ∗ ρ) (subst' f fv e')) →
+    typed_step_ty ρ (Rec f xl e) (fn θ).
+  Proof.
+    iIntros (Hn He tid) "!#(#HEAP&#LFT&#Hρ&$)".
+    assert (Rec f xl e = RecV f xl e) as -> by done. iApply wp_value'.
+    rewrite has_type_value.
+    iLöb as "IH". iExists _. iSplit. done. iIntros (a vl) "!#[Hθ?]".
+    assert (is_Some (subst_l xl (map of_val vl) e)) as [e' He'].
+    { clear -Hn. revert xl Hn e. induction vl=>-[|x xl] //=. by eauto.
+      intros ? e. edestruct IHvl as [e' ->]. congruence. eauto. }
+    iApply wp_rec; try done.
+    { apply List.Forall_forall=>?. rewrite in_map_iff=>-[?[<- _]].
+      rewrite to_of_val. eauto. }
+    iNext. iApply He. done. iFrame "∗#". by rewrite has_type_value.
+  Qed.
+
+  Lemma typed_cont {n} `{Closed (f :b: xl +b+ []) e} ρ θ :
+    length xl = n →
+    (∀ (fv : val) (vl : vec val n) e',
+        subst_l xl (map of_val vl) e = Some e' →
+        typed_program (fv ◁ cont (λ vl, ρ ∗ θ vl)%P ∗ (θ vl) ∗ ρ) (subst' f fv e')) →
+    typed_step_ty ρ (Rec f xl e) (cont θ).
+  Proof.
+    iIntros (Hn He tid) "!#(#HEAP&#LFT&Hρ&$)". specialize (He (RecV f xl e)).
+    assert (Rec f xl e = RecV f xl e) as -> by done. iApply wp_value'.
+    rewrite has_type_value.
+    iLöb as "IH". iExists _. iSplit. done. iIntros (vl) "Hθ ?".
+    assert (is_Some (subst_l xl (map of_val vl) e)) as [e' He'].
+    { clear -Hn. revert xl Hn e. induction vl=>-[|x xl] //=. by eauto.
+      intros ? e. edestruct IHvl as [e' ->]. congruence. eauto. }
+    iApply wp_rec; try done.
+    { apply List.Forall_forall=>?. rewrite in_map_iff=>-[?[<- _]].
+      rewrite to_of_val. eauto. }
+    iNext. iApply He. done. iFrame "∗#". rewrite has_type_value.
+    iExists _. iSplit. done. iIntros (vl') "[Hρ Hθ] Htl".
+    iDestruct ("IH" with "Hρ") as (f') "[Hf' IH']".
+    iDestruct "Hf'" as %[=<-]. iApply ("IH'" with "Hθ Htl").
+  Qed.
+
+End fn.
