theories/typing/int.v
@@ -1,0 +1,54 @@
+From iris.proofmode Require Import tactics.
+From lrust.typing Require Export type.
+From lrust.typing Require Import typing bool.
+
+Section int.
+  Context `{iris_typeG Σ}.
+
+  Program Definition int : type :=
+    {| st_size := 1; st_own tid vl := (∃ z:Z, ⌜vl = [ #z ]⌝)%I |}.
+  Next Obligation. iIntros (tid vl) "H". iDestruct "H" as (z) "%". by subst. Qed.
+
+  Lemma typed_int ρ (z:Datatypes.nat) :
+    typed_step_ty ρ #z int.
+  Proof. iIntros (tid) "!#(_&_&_&$)". wp_value. by iExists _. Qed.
+
+  Lemma typed_plus e1 e2 ρ1 ρ2:
+    typed_step_ty ρ1 e1 int → typed_step_ty ρ2 e2 int →
+    typed_step_ty (ρ1 ∗ ρ2) (e1 + e2) int.
+  Proof.
+    unfold typed_step_ty, typed_step. setoid_rewrite has_type_value.
+    iIntros (He1 He2 tid) "!#(#HEAP&#ĽFT&[H1 H2]&?)".
+    wp_bind e1. iApply wp_wand_r. iSplitR "H2". iApply He1; iFrame "∗#".
+    iIntros (v1) "[Hv1?]". iDestruct "Hv1" as (z1) "Hz1". iDestruct "Hz1" as %[=->].
+    wp_bind e2. iApply wp_wand_r. iSplitL. iApply He2; iFrame "∗#".
+    iIntros (v2) "[Hv2$]". iDestruct "Hv2" as (z2) "Hz2". iDestruct "Hz2" as %[=->].
+    wp_op. by iExists _.
+  Qed.
+
+  Lemma typed_minus e1 e2 ρ1 ρ2:
+    typed_step_ty ρ1 e1 int → typed_step_ty ρ2 e2 int →
+    typed_step_ty (ρ1 ∗ ρ2) (e1 - e2) int.
+  Proof.
+    unfold typed_step_ty, typed_step. setoid_rewrite has_type_value.
+    iIntros (He1 He2 tid) "!#(#HEAP&#LFT&[H1 H2]&?)".
+    wp_bind e1. iApply wp_wand_r. iSplitR "H2". iApply He1; iFrame "∗#".
+    iIntros (v1) "[Hv1?]". iDestruct "Hv1" as (z1) "Hz1". iDestruct "Hz1" as %[=->].
+    wp_bind e2. iApply wp_wand_r. iSplitL. iApply He2; iFrame "∗#".
+    iIntros (v2) "[Hv2$]". iDestruct "Hv2" as (z2) "Hz2". iDestruct "Hz2" as %[=->].
+    wp_op. by iExists _.
+  Qed.
+
+  Lemma typed_le e1 e2 ρ1 ρ2:
+    typed_step_ty ρ1 e1 int → typed_step_ty ρ2 e2 int →
+    typed_step_ty (ρ1 ∗ ρ2) (e1 ≤ e2) bool.
+  Proof.
+    unfold typed_step_ty, typed_step. setoid_rewrite has_type_value.
+    iIntros (He1 He2 tid) "!#(#HEAP&#LFT&[H1 H2]&?)".
+    wp_bind e1. iApply wp_wand_r. iSplitR "H2". iApply He1; iFrame "∗#".
+    iIntros (v1) "[Hv1?]". iDestruct "Hv1" as (z1) "Hz1". iDestruct "Hz1" as %[=->].
+    wp_bind e2. iApply wp_wand_r. iSplitL. iApply He2; iFrame "∗#".
+    iIntros (v2) "[Hv2$]". iDestruct "Hv2" as (z2) "Hz2". iDestruct "Hz2" as %[=->].
+    wp_op; intros _; by iExists _.
+  Qed.
+End int.
