theories/typing/product.v
@@ -1,0 +1,188 @@
+From iris.proofmode Require Import tactics.
+From lrust.lifetime Require Import borrow frac_borrow.
+From lrust.typing Require Export type.
+From lrust.typing Require Import perm type_incl.
+
+Section product.
+  Context `{iris_typeG Σ}.
+
+  Program Definition unit : type :=
+    {| st_size := 0; st_own tid vl := ⌜vl = []⌝%I |}.
+  Next Obligation. iIntros (tid vl) "%". simpl. by subst. Qed.
+
+  Lemma split_prod_mt tid ty1 ty2 q l :
+    (l ↦∗{q}: λ vl,
+       ∃ vl1 vl2, ⌜vl = vl1 ++ vl2⌝ ∗ ty1.(ty_own) tid vl1 ∗ ty2.(ty_own) tid vl2)%I
+       ⊣⊢ l ↦∗{q}: ty1.(ty_own) tid ∗ shift_loc l ty1.(ty_size) ↦∗{q}: ty2.(ty_own) tid.
+  Proof.
+    iSplit; iIntros "H".
+    - iDestruct "H" as (vl) "[H↦ H]". iDestruct "H" as (vl1 vl2) "(% & H1 & H2)".
+      subst. rewrite heap_mapsto_vec_app. iDestruct "H↦" as "[H↦1 H↦2]".
+      iDestruct (ty_size_eq with "H1") as %->.
+      iSplitL "H1 H↦1"; iExists _; iFrame.
+    - iDestruct "H" as "[H1 H2]". iDestruct "H1" as (vl1) "[H↦1 H1]".
+      iDestruct "H2" as (vl2) "[H↦2 H2]". iExists (vl1 ++ vl2).
+      rewrite heap_mapsto_vec_app. iDestruct (ty_size_eq with "H1") as %->.
+      iFrame. iExists _, _. by iFrame.
+  Qed.
+
+  Program Definition product2 (ty1 ty2 : type) :=
+    {| ty_size := ty1.(ty_size) + ty2.(ty_size);
+       ty_own tid vl := (∃ vl1 vl2,
+         ⌜vl = vl1 ++ vl2⌝ ∗ ty1.(ty_own) tid vl1 ∗ ty2.(ty_own) tid vl2)%I;
+       ty_shr κ tid E l :=
+         (∃ E1 E2, ⌜E1 ⊥ E2 ∧ E1 ⊆ E ∧ E2 ⊆ E⌝ ∗
+            ty1.(ty_shr) κ tid E1 l ∗
+            ty2.(ty_shr) κ tid E2 (shift_loc l ty1.(ty_size)))%I |}.
+  Next Obligation.
+    iIntros (ty1 ty2 tid vl) "H". iDestruct "H" as (vl1 vl2) "(% & H1 & H2)".
+    subst. rewrite app_length !ty_size_eq.
+    iDestruct "H1" as %->. iDestruct "H2" as %->. done.
+  Qed.
+  Next Obligation.
+    intros ty1 ty2 E N κ l tid q ??. iIntros "#LFT /=H Htok".
+    rewrite split_prod_mt.
+    iMod (bor_sep with "LFT H") as "[H1 H2]". set_solver.
+    iMod (ty1.(ty_share) _ (N .@ 1) with "LFT H1 Htok") as "[? Htok]". solve_ndisj. done.
+    iMod (ty2.(ty_share) _ (N .@ 2) with "LFT H2 Htok") as "[? $]". solve_ndisj. done.
+    iModIntro. iExists (↑N .@ 1). iExists (↑N .@ 2). iFrame.
+    iPureIntro. split. solve_ndisj. split; apply nclose_subseteq.
+  Qed.
+  Next Obligation.
+    intros ty1 ty2 κ κ' tid E E' l ?. iIntros "#LFT /= #H⊑ H".
+    iDestruct "H" as (N1 N2) "(% & H1 & H2)". iExists N1, N2.
+    iSplit. iPureIntro. set_solver.
+    iSplitL "H1"; by iApply (ty_shr_mono with "LFT H⊑").
+  Qed.
+
+  Global Program Instance product2_copy `(!Copy ty1) `(!Copy ty2) :
+    Copy (product2 ty1 ty2).
+  Next Obligation.
+    intros ty1 ? ty2 ? κ tid E F l q ?. iIntros "#LFT H [[Htok1 Htok2] Htl]".
+    iDestruct "H" as (E1 E2) "(% & H1 & H2)".
+    assert (F = E1 ∪ E2 ∪ F∖(E1 ∪ E2)) as ->.
+    { rewrite -union_difference_L; set_solver. }
+    repeat setoid_rewrite na_own_union; first last.
+    set_solver. set_solver. set_solver. set_solver.
+    iDestruct "Htl" as "[[Htl1 Htl2] $]".
+    iMod (@copy_shr_acc with "LFT H1 [$Htok1 $Htl1]") as (q1) "[H1 Hclose1]". set_solver.
+    iMod (@copy_shr_acc with "LFT H2 [$Htok2 $Htl2]") as (q2) "[H2 Hclose2]". set_solver.
+    destruct (Qp_lower_bound q1 q2) as (qq & q'1 & q'2 & -> & ->). iExists qq.
+    iDestruct "H1" as (vl1) "[H↦1 H1]". iDestruct "H2" as (vl2) "[H↦2 H2]".
+    rewrite !split_prod_mt.
+    iAssert (▷ ⌜length vl1 = ty1.(ty_size)⌝)%I with "[#]" as ">%".
+    { iNext. by iApply ty_size_eq. }
+    iAssert (▷ ⌜length vl2 = ty2.(ty_size)⌝)%I with "[#]" as ">%".
+    { iNext. by iApply ty_size_eq. }
+    iDestruct "H↦1" as "[H↦1 H↦1f]". iDestruct "H↦2" as "[H↦2 H↦2f]".
+    iIntros "!>". iSplitL "H↦1 H1 H↦2 H2".
+    - iNext. iSplitL "H↦1 H1". iExists vl1. by iFrame. iExists vl2. by iFrame.
+    - iIntros "[H1 H2]".
+      iDestruct "H1" as (vl1') "[H↦1 H1]". iDestruct "H2" as (vl2') "[H↦2 H2]".
+      iAssert (▷ ⌜length vl1' = ty1.(ty_size)⌝)%I with "[#]" as ">%".
+      { iNext. by iApply ty_size_eq. }
+      iAssert (▷ ⌜length vl2' = ty2.(ty_size)⌝)%I with "[#]" as ">%".
+      { iNext. by iApply ty_size_eq. }
+      iCombine "H↦1" "H↦1f" as "H↦1". iCombine "H↦2" "H↦2f" as "H↦2".
+      rewrite !heap_mapsto_vec_op; try by congruence.
+      iDestruct "H↦1" as "[_ H↦1]". iDestruct "H↦2" as "[_ H↦2]".
+      iMod ("Hclose1" with "[H1 H↦1]") as "[$$]". by iExists _; iFrame.
+      iMod ("Hclose2" with "[H2 H↦2]") as "[$$]". by iExists _; iFrame. done.
+  Qed.
+
+  Definition product := fold_right product2 unit.
+End product.
+
+Arguments product : simpl never.
+Notation Π := product.
+
+Section typing.
+  Context `{iris_typeG Σ}.
+
+  (* We have the additional hypothesis that ρ should be duplicable.
+     The only way I can see to circumvent this limitation is to deeply
+     embed permissions (and their inclusion). Not sure this is worth it. *)
+  Lemma ty_incl_prod2 ρ ty11 ty12 ty21 ty22 :
+    Duplicable ρ → ty_incl ρ ty11 ty12 → ty_incl ρ ty21 ty22 →
+    ty_incl ρ (product2 ty11 ty21) (product2 ty12 ty22).
+  Proof.
+    iIntros (Hρ Hincl1 Hincl2 tid) "#LFT #Hρ".
+    iMod (Hincl1 with "LFT Hρ") as "[#Ho1#Hs1]".
+    iMod (Hincl2 with "LFT Hρ") as "[#Ho2#Hs2]".
+    iSplitL; iIntros "!>!#*H/=".
+    - iDestruct "H" as (vl1 vl2) "(% & H1 & H2)". iExists _, _. iSplit. done.
+      iSplitL "H1". iApply ("Ho1" with "H1"). iApply ("Ho2" with "H2").
+    - iDestruct "H" as (E1 E2) "(% & H1 & H2)".
+      iDestruct ("Hs1" with "*H1") as "[H1 EQ]". iDestruct ("Hs2" with "*H2") as "[H2 %]".
+      iDestruct "EQ" as %->. iSplit; last by iPureIntro; f_equal.
+      iExists _, _. by iFrame.
+  Qed.
+
+  Lemma ty_incl_prod ρ tyl1 tyl2 :
+    Duplicable ρ → Forall2 (ty_incl ρ) tyl1 tyl2 → ty_incl ρ (Π tyl1) (Π tyl2).
+  Proof. intros Hρ HFA. induction HFA. done. by apply ty_incl_prod2. Qed.
+
+  Lemma ty_incl_prod2_assoc1 ρ ty1 ty2 ty3 :
+    ty_incl ρ (product2 ty1 (product2 ty2 ty3)) (product2 (product2 ty1 ty2) ty3).
+  Proof.
+    iIntros (tid) "_ _!>". iSplit; iIntros "!#/=*H".
+    - iDestruct "H" as (vl1 vl') "(% & Ho1 & H)".
+      iDestruct "H" as (vl2 vl3) "(% & Ho2 & Ho3)". subst.
+      iExists _, _. iSplit. by rewrite assoc. iFrame. iExists _, _. by iFrame.
+    - iDestruct "H" as (E1 E2') "(% & Hs1 & H)".
+      iDestruct "H" as (E2 E3) "(% & Hs2 & Hs3)". rewrite shift_loc_assoc_nat.
+      iSplit; last by rewrite assoc.
+      iExists (E1 ∪ E2), E3. iSplit. by iPureIntro; set_solver. iFrame.
+      iExists E1, E2. iSplit. by iPureIntro; set_solver. by iFrame.
+  Qed.
+
+  Lemma ty_incl_prod2_assoc2 ρ ty1 ty2 ty3 :
+    ty_incl ρ (product2 (product2 ty1 ty2) ty3) (product2 ty1 (product2 ty2 ty3)).
+  Proof.
+    iIntros (tid) "_ _!>". iSplit; iIntros "!#/=*H".
+    - iDestruct "H" as (vl1 vl') "(% & H & Ho3)".
+      iDestruct "H" as (vl2 vl3) "(% & Ho1 & Ho2)". subst.
+      iExists _, _. iSplit. by rewrite -assoc. iFrame. iExists _, _. by iFrame.
+    - iDestruct "H" as (E1' E3) "(% & H & Hs3)".
+      iDestruct "H" as (E1 E2) "(% & Hs1 & Hs2)". rewrite shift_loc_assoc_nat.
+      iSplit; last by rewrite assoc.
+      iExists E1, (E2 ∪ E3). iSplit. by iPureIntro; set_solver. iFrame.
+      iExists E2, E3. iSplit. by iPureIntro; set_solver. by iFrame.
+  Qed.
+
+  Lemma ty_incl_prod_flatten ρ tyl1 tyl2 tyl3 :
+    ty_incl ρ (Π(tyl1 ++ Π tyl2 :: tyl3))
+              (Π(tyl1 ++ tyl2 ++ tyl3)).
+  Proof.
+    apply (ty_incl_weaken _ ⊤). apply perm_incl_top.
+    induction tyl1; last by apply (ty_incl_prod2 _ _ _ _ _ _).
+    induction tyl2 as [|ty tyl2 IH]; simpl.
+    - iIntros (tid) "#LFT _". iSplitL; iIntros "/=!>!#*H".
+      + iDestruct "H" as (vl1 vl2) "(% & % & Ho)". subst. done.
+      + iDestruct "H" as (E1 E2) "(% & H1 & Ho)". iSplit; last done.
+        rewrite shift_loc_0. iApply (ty_shr_mono with "LFT [] Ho"). set_solver.
+        iApply lft_incl_refl.
+    - etransitivity. apply ty_incl_prod2_assoc2.
+      eapply (ty_incl_prod2 _ _ _ _ _ _). done. apply IH.
+  Qed.
+
+  Lemma ty_incl_prod_unflatten ρ tyl1 tyl2 tyl3 :
+    ty_incl ρ (Π(tyl1 ++ tyl2 ++ tyl3))
+              (Π(tyl1 ++ Π tyl2 :: tyl3)).
+  Proof.
+    apply (ty_incl_weaken _ ⊤). apply perm_incl_top.
+    induction tyl1; last by apply (ty_incl_prod2 _ _ _ _ _ _).
+    induction tyl2 as [|ty tyl2 IH]; simpl.
+    - iIntros (tid) "#LFT _". iMod (bor_create with "LFT []") as "[Hbor _]".
+      done. instantiate (1:=True%I). by auto. instantiate (1:=static).
+      iMod (bor_fracture (λ _, True%I) with "LFT Hbor") as "#Hbor". done.
+      iSplitL; iIntros "/=!>!#*H".
+      + iExists [], vl. iFrame. auto.
+      + iSplit; last done. iExists ∅, E. iSplit. iPureIntro; set_solver.
+        rewrite shift_loc_0. iFrame. iExists []. iSplit; last auto.
+        setoid_rewrite heap_mapsto_vec_nil.
+        iApply (frac_bor_shorten with "[] Hbor"). iApply lft_incl_static.
+    - etransitivity; last apply ty_incl_prod2_assoc1.
+      eapply (ty_incl_prod2 _ _ _ _ _ _). done. apply IH.
+  Qed.
+End typing.
