theories/typing/sum.v
@@ -1,0 +1,160 @@
+From iris.proofmode Require Import tactics.
+From lrust.lifetime Require Import borrow frac_borrow.
+From lrust.typing Require Export type.
+From lrust.typing Require Import type_incl.
+
+Section sum.
+  Context `{iris_typeG Σ}.
+
+  (* [emp] cannot be defined using [ty_of_st], because the least we
+     would be able to prove from its [ty_shr] would be [▷ False], but
+     we really need [False] to prove [ty_incl_emp]. *)
+  Program Definition emp :=
+    {| ty_size := 0; ty_own tid vl := False%I; ty_shr κ tid E l := False%I |}.
+  Next Obligation. iIntros (tid vl) "[]". Qed.
+  Next Obligation.
+    iIntros (????????) "#LFT Hb Htok".
+    iMod (bor_exists with "LFT Hb") as (vl) "Hb". set_solver.
+    iMod (bor_sep with "LFT Hb") as "[_ Hb]". set_solver.
+    iMod (bor_persistent with "LFT Hb Htok") as "[>[] _]". set_solver.
+  Qed.
+  Next Obligation. intros. iIntros "_ _ []". Qed.
+  Global Instance emp_empty : Empty type := emp.
+
+  Global Program Instance emp_copy : Copy emp.
+  Next Obligation. intros. iIntros "_ []". Qed.
+
+  Lemma split_sum_mt l tid q tyl :
+    (l ↦∗{q}: λ vl,
+         ∃ (i : nat) vl', ⌜vl = #i :: vl'⌝ ∗ ty_own (nth i tyl ∅) tid vl')%I
+    ⊣⊢ ∃ (i : nat), l ↦{q} #i ∗ shift_loc l 1 ↦∗{q}: ty_own (nth i tyl ∅) tid.
+  Proof.
+    iSplit; iIntros "H".
+    - iDestruct "H" as (vl) "[Hmt Hown]". iDestruct "Hown" as (i vl') "[% Hown]".
+      subst. iExists i. iDestruct (heap_mapsto_vec_cons with "Hmt") as "[$ Hmt]".
+      iExists vl'. by iFrame.
+    - iDestruct "H" as (i) "[Hmt1 Hown]". iDestruct "Hown" as (vl) "[Hmt2 Hown]".
+      iExists (#i::vl). rewrite heap_mapsto_vec_cons. iFrame. eauto.
+  Qed.
+
+  Class LstTySize (n : nat) (tyl : list type) :=
+    size_eq : Forall ((= n) ∘ ty_size) tyl.
+  Instance LstTySize_nil n : LstTySize n nil := List.Forall_nil _.
+  Lemma LstTySize_cons n ty tyl :
+    ty.(ty_size) = n → LstTySize n tyl → LstTySize n (ty :: tyl).
+  Proof. intros. constructor; done. Qed.
+
+  Lemma sum_size_eq n tid i tyl vl {Hn : LstTySize n tyl} :
+    ty_own (nth i tyl ∅) tid vl -∗ ⌜length vl = n⌝.
+  Proof.
+    iIntros "Hown". iDestruct (ty_size_eq with "Hown") as %->.
+    revert Hn. rewrite /LstTySize List.Forall_forall /= =>Hn.
+    edestruct nth_in_or_default as [| ->]. by eauto.
+    iDestruct "Hown" as "[]".
+  Qed.
+
+  Program Definition sum {n} (tyl : list type) {_:LstTySize n tyl} :=
+    {| ty_size := S n;
+       ty_own tid vl :=
+         (∃ (i : nat) vl', ⌜vl = #i :: vl'⌝ ∗ (nth i tyl ∅).(ty_own) tid vl')%I;
+       ty_shr κ tid N l :=
+         (∃ (i : nat), (&frac{κ} λ q, l ↦{q} #i) ∗
+               (nth i tyl ∅).(ty_shr) κ tid N (shift_loc l 1))%I
+    |}.
+  Next Obligation.
+    iIntros (n tyl Hn tid vl) "Hown". iDestruct "Hown" as (i vl') "(%&Hown)".
+    subst. simpl. by iDestruct (sum_size_eq with "Hown") as %->.
+  Qed.
+  Next Obligation.
+    intros n tyl Hn E N κ l tid q ??. iIntros "#LFT Hown Htok". rewrite split_sum_mt.
+    iMod (bor_exists with "LFT Hown") as (i) "Hown". set_solver.
+    iMod (bor_sep with "LFT Hown") as "[Hmt Hown]". set_solver.
+    iMod ((nth i tyl ∅).(ty_share) with "LFT Hown Htok") as "[#Hshr $]"; try done.
+    iMod (bor_fracture with "LFT [-]") as "H"; last by eauto. set_solver. iFrame.
+  Qed.
+  Next Obligation.
+    intros n tyl Hn κ κ' tid E E' l ?. iIntros "#LFT #Hord H".
+    iDestruct "H" as (i) "[Hown0 Hown]". iExists i. iSplitL "Hown0".
+    by iApply (frac_bor_shorten with "Hord").
+    iApply ((nth i tyl ∅).(ty_shr_mono) with "LFT Hord"); last done. done.
+  Qed.
+
+  (* TODO : Make the Forall parameter a typeclass *)
+  Global Program Instance sum_copy `(LstTySize n tyl) :
+    Forall Copy tyl → Copy (sum tyl).
+  Next Obligation.
+    intros n tyl Hn HFA tid vl.
+    cut (∀ i vl', PersistentP (ty_own (nth i tyl ∅) tid vl')). by apply _.
+    intros. apply @copy_persistent. edestruct nth_in_or_default as [| ->];
+      [by eapply List.Forall_forall| apply _].
+  Qed.
+  Next Obligation.
+    intros n tyl Hn HFA κ tid E F l q ?.
+    iIntros "#LFT #H[[Htok1 Htok2] Htl]".
+    setoid_rewrite split_sum_mt. iDestruct "H" as (i) "[Hshr0 Hshr]".
+    iMod (frac_bor_acc with "LFT Hshr0 Htok1") as (q'1) "[Hown Hclose]". set_solver.
+    iMod (@copy_shr_acc _ _ (nth i tyl ∅) with "LFT Hshr [Htok2 $Htl]")
+      as (q'2) "[Hownq Hclose']"; try done.
+    { edestruct nth_in_or_default as [| ->]; last by apply _.
+        by eapply List.Forall_forall. }
+    destruct (Qp_lower_bound q'1 q'2) as (q' & q'01 & q'02 & -> & ->).
+    rewrite -{1}heap_mapsto_vec_prop_op; last (by intros; apply sum_size_eq, Hn).
+    iDestruct "Hownq" as "[Hownq1 Hownq2]". iDestruct "Hown" as "[Hown1 Hown2]".
+    iExists q'. iModIntro. iSplitL "Hown1 Hownq1".
+    - iNext. iExists i. by iFrame.
+    - iIntros "H". iDestruct "H" as (i') "[Hown1 Hownq1]".
+      iCombine "Hown1" "Hown2" as "Hown". rewrite heap_mapsto_op.
+      iDestruct "Hown" as "[>#Hi Hown]". iDestruct "Hi" as %[= ->%Z_of_nat_inj].
+      iMod ("Hclose" with "Hown") as "$".
+      iCombine "Hownq1" "Hownq2" as "Hownq".
+      rewrite heap_mapsto_vec_prop_op; last (by intros; apply sum_size_eq, Hn).
+      by iApply "Hclose'".
+  Qed.
+
+End sum.
+
+Existing Instance LstTySize_nil.
+Hint Extern 1 (LstTySize _ (_ :: _)) =>
+  apply LstTySize_cons; [compute; reflexivity|] : typeclass_instances.
+
+
+(* Σ is commonly used for the current functor. So it cannot be defined
+   as Π for products. We stick to the following form. *)
+Notation "Σ[ ty1 ; .. ; tyn ]" :=
+  (sum (cons ty1 (..(cons tyn nil)..))) : lrust_type_scope.
+
+Section incl.
+  Context `{iris_typeG Σ}.
+
+  Lemma ty_incl_emp ρ ty : ty_incl ρ ∅ ty.
+  Proof. iIntros (tid) "_ _!>". iSplit; iIntros "!#*/=[]". Qed.
+
+  Lemma ty_incl_sum ρ n tyl1 tyl2 (_ : LstTySize n tyl1) (_ : LstTySize n tyl2) :
+    Duplicable ρ → Forall2 (ty_incl ρ) tyl1 tyl2 →
+    ty_incl ρ (sum tyl1) (sum tyl2).
+  Proof.
+    iIntros (DUP FA tid) "#LFT #Hρ". rewrite /sum /=. iSplitR "".
+    - assert (Hincl : lft_ctx -∗ ρ tid ={⊤}=∗
+         (□ ∀ i vl, (nth i tyl1 ∅%T).(ty_own) tid vl
+                  → (nth i tyl2 ∅%T).(ty_own) tid vl)).
+      { clear -FA DUP. induction FA as [|ty1 ty2 tyl1 tyl2 Hincl _ IH].
+        - iIntros "_ _!>*!#". eauto.
+        - iIntros "#LFT #Hρ". iMod (IH with "LFT Hρ") as "#IH".
+          iMod (Hincl with "LFT Hρ") as "[#Hh _]".
+          iIntros "!>*!#*Hown". destruct i as [|i]. by iApply "Hh". by iApply "IH". }
+      iMod (Hincl with "LFT Hρ") as "#Hincl". iIntros "!>!#*H".
+      iDestruct "H" as (i vl') "[% Hown]". subst. iExists _, _. iSplit. done.
+        by iApply "Hincl".
+    - assert (Hincl : lft_ctx -∗ ρ tid ={⊤}=∗
+         (□ ∀ i κ E l, (nth i tyl1 ∅%T).(ty_shr) κ tid E l
+                     → (nth i tyl2 ∅%T).(ty_shr) κ tid E l)).
+      { clear -FA DUP. induction FA as [|ty1 ty2 tyl1 tyl2 Hincl _ IH].
+        - iIntros "#LFT _!>*!#". eauto.
+        - iIntros "#LFT #Hρ".
+          iMod (IH with "LFT Hρ") as "#IH". iMod (Hincl with "LFT Hρ") as "[_ #Hh]".
+          iIntros "!>*!#*Hown". destruct i as [|i]; last by iApply "IH".
+          by iDestruct ("Hh" $! _ _ _ with "Hown") as "[$ _]". }
+      iMod (Hincl with "LFT Hρ") as "#Hincl". iIntros "!>!#*H". iSplit; last done.
+      iDestruct "H" as (i) "[??]". iExists _. iSplit. done. by iApply "Hincl".
+  Qed.
+End incl.
